Some more changes

coq/theories/functional/FunSyntax.v
@@ -1,6 +1,9 @@
+From impboot Require Import utils.Core.
 From Stdlib Require Import NArith.
 From Stdlib Require Import Lists.List.
 Import ListNotations.
+
+Open Scope N.
 
 Notation name := N (only parsing).
 
@@ -19,101 +22,30 @@ Inductive test : Type :=
 | Equal.
 
 Inductive exp : Type :=
-| Const (n : N)                                  (* constant number            *)
-| Var (n : name)                                 (* local variable             *)
-| Op (o : op) (args : list exp)                  (* primitive operations       *)
-| If (t : test) (conds : list exp) (e1 e2 : exp) (* if test .. then .. else .. *)
-| Let (n : name) (e1 e2 : exp)                   (* let name = .. in ..        *)
-| Call (f : name) (args : list exp).             (* call a function            *)
+| Const (n: N)                                 (* constant number            *)
+| Var (n: name)                                (* local variable             *)
+| Op (o: op) (args: list exp)                  (* primitive operations       *)
+| If (t: test) (conds: list exp) (e1 e2: exp)  (* if test .. then .. else .. *)
+| Let (n: name) (e1 e2: exp)                   (* let name = .. in ..        *)
+| Call (f: name) (args: list exp).             (* call a function            *)
 
-Fixpoint exp_ind_str (P : exp -> Prop)
-  (HConst : forall n : N, P (Const n))
-  (HVar : forall n : name, P (Var n))
-  (HOp : forall (o : op) (args : list exp), Forall P args -> P (Op o args))
-  (HIf : forall (t : test) (conds : list exp) (e1 e2 : exp),
-      Forall P conds -> P e1 -> P e2 -> P (If t conds e1 e2))
-  (HLet : forall (n : name) (e1 e2 : exp), P e1 -> P e2 -> P (Let n e1 e2))
-  (HCall : forall (f : name) (args : list exp), Forall P args -> P (Call f args))
-  (e : exp) : P e :=
-  match e as e0 return P e0 with
-  | Const n =>
-    HConst n
-  | Var n =>
-    HVar n
-  | Op o args =>
-    HOp o args ((fix list_exp_ind (l : list exp) : Forall P l :=
-                  match l with
-                  | [] => Forall_nil P
-                  | e :: l' => Forall_cons e (exp_ind_str P HConst HVar HOp HIf HLet HCall e)
-                                      (list_exp_ind l')
-                  end) args)
-  | If t conds e1 e2 =>
-    HIf t conds e1 e2 ((fix list_exp_ind (l : list exp) : Forall P l :=
-                          match l with
-                          | [] => Forall_nil P
-                          | e :: l' => Forall_cons e (exp_ind_str P HConst HVar HOp HIf HLet HCall e)
-                                                (list_exp_ind l')
-                          end) conds) (exp_ind_str P HConst HVar HOp HIf HLet HCall e1)
-                          (exp_ind_str P HConst HVar HOp HIf HLet HCall e2)
-  | Let n e1 e2 =>
-    HLet n e1 e2 (exp_ind_str P HConst HVar HOp HIf HLet HCall e1)
-                 (exp_ind_str P HConst HVar HOp HIf HLet HCall e2)
-  | Call f args =>
-    HCall f args ((fix list_exp_ind (l : list exp) : Forall P l :=
-                    match l with
-                    | [] => Forall_nil P
-                    | e :: l' => Forall_cons e (exp_ind_str P HConst HVar HOp HIf HLet HCall e)
-                                          (list_exp_ind l')
-                    end) args)
-  end.
-
-(* Not decreasing *)
-Fail Fixpoint exp_ind_list (P : list exp -> Prop)
-  (HNil : P [])
-  (HCons : forall e es, P [e] -> P es -> P (e :: es))
-  (HConst : forall n : N, P [Const n])
-  (HVar : forall n : name, P [Var n])
-  (HOp : forall (o : op) (args : list exp), P args -> P [Op o args])
-  (HIf : forall (t : test) (conds : list exp) (e1 e2 : exp),
-      P conds -> P [e1] -> P [e2] -> P [If t conds e1 e2])
-  (HLet : forall (n : name) (e1 e2 : exp), P [e1] -> P [e2] -> P [Let n e1 e2])
-  (HCall : forall (f : name) (args : list exp), P args -> P [Call f args])
-  (es : list exp) : P es :=
-  match es with
-  | [] => HNil
-  | [Const n] => HConst n
-  | [Var n] => HVar n
-  | [Op o args] =>
-    HOp o args (exp_ind_list P HNil HCons HConst HVar HOp HIf HLet HCall args)
-  | [If t conds e1 e2] =>
-    HIf t conds e1 e2 (exp_ind_list P HNil HCons HConst HVar HOp HIf HLet HCall conds)
-                      (exp_ind_list P HNil HCons HConst HVar HOp HIf HLet HCall [e1])
-                      (exp_ind_list P HNil HCons HConst HVar HOp HIf HLet HCall [e2])
-  | [Let n e1 e2] =>
-    HLet n e1 e2 (exp_ind_list P HNil HCons HConst HVar HOp HIf HLet HCall [e1])
-                 (exp_ind_list P HNil HCons HConst HVar HOp HIf HLet HCall [e2])
-  | [Call f args] =>
-    HCall f args (exp_ind_list P HNil HCons HConst HVar HOp HIf HLet HCall args)
-  | e :: es' =>
-    HCons e es'
-           (exp_ind_list P HNil HCons HConst HVar HOp HIf HLet HCall [e])
-           (exp_ind_list P HNil HCons HConst HVar HOp HIf HLet HCall es')
-  end.
-
-Inductive dec : Type :=
-| Defun (n : name) (params : list name) (body : exp). (* func name, formal params, body *)
+Inductive defun: Type :=
+| Defun (n: name) (params: list name) (body: exp). (* func name, formal params, body *)
 
 (* a complete program is a list of function declarations followed by *)
 (* an expression to evaluate *)
-Inductive prog : Type :=
-| Program (defs : list dec) (main : exp).
+Inductive prog: Type :=
+| Program (defs: list defun) (main: exp).
 
-Definition get_main (p : prog) : exp :=
+Definition get_main (p: prog): exp :=
   match p with
   | Program _ main => main
   end.
 
-Definition get_defs (p : prog) : list dec :=
+Definition get_defs (p: prog): list defun :=
   match p with
   | Program defs _ => defs
   end.
+
+Definition name_of_string_N (s: string): N :=
+  fold_right (fun c acc => (N_of_ascii c) * 256 + acc) 0 (list_ascii_of_string s).
