coq/theories/fp2imp/FpToImpCodegen.v
@@ -1,0 +1,254 @@
+From impboot Require Import functional.FunSyntax.
+From impboot Require Import imperative.ImpSyntax.
+From Stdlib Require Import NArith.
+From Stdlib Require Import ZArith.
+From Stdlib Require Import Lists.List.
+From Stdlib Require Import Bool.
+From Stdlib Require Import String.
+Require Import coqutil.Word.Interface.
+Require Import coqutil.Word.Properties.
+Require Import coqutil.Datatypes.List.
+Import ListNotations.
+
+(* definition of a very partial compilation from functional to imperative source *)
+
+Open Scope string_scope.
+
+Definition option_bind {A B: Type} (f: A -> option B) (ma: option A): option B :=
+  match ma with
+  | None => None
+  | Some a => f a
+  end.
+
+Notation "'let/o' v := r1 'in' r2" :=
+  (option_bind (fun v => r2) r1)
+  (at level 200, right associativity).
+
+Fixpoint to_exp (e: FunSyntax.exp): option ImpSyntax.exp :=
+  match e with
+  | FunSyntax.Var v => Some (ImpSyntax.Var (N.to_nat v))
+  | FunSyntax.Const n =>
+      if (n <? 2^64)%N then
+        Some (ImpSyntax.Const (word.of_Z (Z.of_N n)))
+      else None
+  | FunSyntax.Op FunSyntax.Head [x] =>
+      option_map (fun e' => ImpSyntax.Read e' (ImpSyntax.Const (word.of_Z 0))) (to_exp x)
+  | FunSyntax.Op FunSyntax.Tail [x] =>
+      option_map (fun e' => ImpSyntax.Read e' (ImpSyntax.Const (word.of_Z 8))) (to_exp x)
+  | _ => None
+  end.
+
+Fixpoint to_exps (es: list FunSyntax.exp): option (list ImpSyntax.exp) :=
+  match es with
+  | [] => Some []
+  | x :: xs =>
+    let/o y := to_exp x in
+    let/o ys := to_exps xs in
+    Some (y :: ys)
+  end.
+
+Definition to_test (t: FunSyntax.test): ImpSyntax.cmp :=
+  match t with
+  | FunSyntax.Equal => ImpSyntax.Equal
+  | FunSyntax.Less => ImpSyntax.Less
+  end.
+
+Definition to_guard (t: FunSyntax.test) (es: list FunSyntax.exp): option ImpSyntax.test :=
+  match to_exps es with
+  | Some [x1; x2] => Some (ImpSyntax.Test (to_test t) x1 x2)
+  | _ => None
+  end.
+
+Definition dest_Cons (e: FunSyntax.exp): option (ImpSyntax.exp * FunSyntax.exp) :=
+  match e with
+  | FunSyntax.Op FunSyntax.Cons [e1; e2] =>
+      option_map (fun e' => (e', e2)) (to_exp e1)
+  | _ => None
+  end.
+
+(* TODO: is this just an optimization? *)
+Definition to_cons (v: name) (x: FunSyntax.exp): option ImpSyntax.cmd :=
+  match dest_Cons x with
+  | None => None
+  | Some (e1, x) =>
+      match dest_Cons x with
+      | None =>
+          option_map (fun e2 => ImpSyntax.Call v (name_of_string "cons") [e1; e2]) (to_exp x)
+      | Some (e2, x) =>
+          match dest_Cons x with
+          | None =>
+              option_map (fun e3 => ImpSyntax.Call v (name_of_string "cons3") [e1; e2; e3]) (to_exp x)
+          | Some (e3, x) =>
+              match dest_Cons x with
+              | None =>
+                  option_map (fun e4 => ImpSyntax.Call v (name_of_string "cons4") [e1; e2; e3; e4]) (to_exp x)
+              | Some (e4, x) =>
+                  option_map (fun e5 => ImpSyntax.Call v (name_of_string "cons5") [e1; e2; e3; e4; e5]) (to_exp x)
+              end
+          end
+      end
+  end.
+
+Definition to_assign (v: name) (x: FunSyntax.exp): option ImpSyntax.cmd :=
+  match to_exp x with
+  | Some i => Some (ImpSyntax.Assign v i)
+  | None =>
+      match to_cons v x with
+      | Some r => Some r
+      | None =>
+          match x with
+          | FunSyntax.Call n es =>
+              option_map (fun xs => ImpSyntax.Call v (N.to_nat n) xs) (to_exps es)
+          | FunSyntax.Op p es =>
+              match p, to_exps es with
+              | FunSyntax.Add, Some [x1; x2] => 
+                  Some (ImpSyntax.Call v (name_of_string "add") [x1; x2])
+              | FunSyntax.Sub, Some [x1; x2] => 
+                  Some (ImpSyntax.Call v (name_of_string "sub") [x1; x2])
+              | FunSyntax.Div, Some [x1; x2] => 
+                  Some (ImpSyntax.Assign v (ImpSyntax.Div x1 x2))
+              | FunSyntax.Read, Some [] => 
+                  Some (ImpSyntax.GetChar v)
+              | FunSyntax.Write, Some [x1] => 
+                  Some (ImpSyntax.Seq (ImpSyntax.PutChar x1) 
+                                      (ImpSyntax.Assign v (ImpSyntax.Const (word.of_Z 0))))
+              | _, _ => None
+              end
+          | _ => None
+          end
+      end
+  end.
+
+Fixpoint to_cmd (e: FunSyntax.exp): option ImpSyntax.cmd :=
+  match to_exp e with
+  | Some i => Some (ImpSyntax.Return i)
+  | None =>
+      match e with
+      | FunSyntax.If t es e1 e2 =>
+          let/o t1 := to_guard t es in
+          let/o c1 := to_cmd e1 in
+          let/o c2 := to_cmd e2 in
+          Some (ImpSyntax.If t1 c1 c2)
+      | FunSyntax.Let v x y =>
+          let/o c1 := to_assign (N.to_nat v) x in
+          let/o c2 := to_cmd y in
+          Some (ImpSyntax.Seq c1 c2)
+      | FunSyntax.Call n es =>
+          option_map (fun xs => 
+            ImpSyntax.Seq 
+              (ImpSyntax.Call (name_of_string "ret") (N.to_nat n) xs) 
+              (ImpSyntax.Return (ImpSyntax.Var (name_of_string "ret")))
+          ) (to_exps es)
+      | _ => None
+      end
+  end.
+
+  Fixpoint list_uniqb {A: Type} (eqb: A -> A -> bool) (l: list A): bool :=
+    match l with
+    | [] => true
+    | x :: xs => negb (List.existsb (eqb x) xs) && list_uniqb eqb xs
+    end.
+
+Fixpoint to_funs (fs: list FunSyntax.defun): option (list ImpSyntax.func) :=
+  match fs with
+  | [] => Some []
+  | FunSyntax.Defun n vs e :: fs =>
+    if list_uniqb N.eqb vs then
+      let/o cmd := to_cmd e in
+      let/o funs := to_funs fs in
+      Some (ImpSyntax.Func (N.to_nat n) (map N.to_nat vs) cmd :: funs)
+    else
+      None
+  end.
+
+Fixpoint list_Seq (cs: list ImpSyntax.cmd): ImpSyntax.cmd :=
+  match cs with
+  | [] => ImpSyntax.Skip
+  | [x] => x
+  | x :: xs => ImpSyntax.Seq x (list_Seq xs)
+  end.
+
+Definition builtin: list (name * list name * ImpSyntax.cmd) :=
+  [(name_of_string "add", [name_of_string "a"; name_of_string "b"], list_Seq
+     [ImpSyntax.Assign (name_of_string "c") 
+        (ImpSyntax.Add (ImpSyntax.Var (name_of_string "a")) (ImpSyntax.Var (name_of_string "b")));
+      ImpSyntax.If (ImpSyntax.Test ImpSyntax.Less (ImpSyntax.Var (name_of_string "c")) 
+                                    (ImpSyntax.Var (name_of_string "a"))) 
+        ImpSyntax.Abort ImpSyntax.Skip;
+      ImpSyntax.If (ImpSyntax.Test ImpSyntax.Less (ImpSyntax.Var (name_of_string "c")) 
+                                    (ImpSyntax.Var (name_of_string "b"))) 
+        ImpSyntax.Abort ImpSyntax.Skip;
+      ImpSyntax.Return (ImpSyntax.Var (name_of_string "c"))]);
+   (name_of_string "sub", [name_of_string "a"; name_of_string "b"], list_Seq
+     [ImpSyntax.If (ImpSyntax.Test ImpSyntax.Less (ImpSyntax.Var (name_of_string "a")) 
+                                    (ImpSyntax.Var (name_of_string "b")))
+        (ImpSyntax.Return (ImpSyntax.Const (word.of_Z 0)))
+        (ImpSyntax.Return (ImpSyntax.Sub (ImpSyntax.Var (name_of_string "a")) 
+                                          (ImpSyntax.Var (name_of_string "b"))))]);
+   (name_of_string "cons", [name_of_string "a"; name_of_string "b"], list_Seq
+     [ImpSyntax.Alloc (name_of_string "ret") (ImpSyntax.Const (word.of_Z 16));
+      ImpSyntax.Update (ImpSyntax.Var (name_of_string "ret")) (ImpSyntax.Const (word.of_Z 0)) 
+                       (ImpSyntax.Var (name_of_string "a"));
+      ImpSyntax.Update (ImpSyntax.Var (name_of_string "ret")) (ImpSyntax.Const (word.of_Z 8)) 
+                       (ImpSyntax.Var (name_of_string "b"));
+      ImpSyntax.Return (ImpSyntax.Var (name_of_string "ret"))]);
+   (name_of_string "cons3", [name_of_string "a"; name_of_string "b"; name_of_string "c"], list_Seq
+     [ImpSyntax.Call (name_of_string "ret") (name_of_string "cons") 
+        [ImpSyntax.Var (name_of_string "b"); ImpSyntax.Var (name_of_string "c")];
+      ImpSyntax.Call (name_of_string "ret") (name_of_string "cons") 
+        [ImpSyntax.Var (name_of_string "a"); ImpSyntax.Var (name_of_string "ret")];
+      ImpSyntax.Return (ImpSyntax.Var (name_of_string "ret"))]);
+   (name_of_string "cons4", [name_of_string "a"; name_of_string "b"; name_of_string "c"; name_of_string "d"], list_Seq
+     [ImpSyntax.Call (name_of_string "ret") (name_of_string "cons3") 
+        [ImpSyntax.Var (name_of_string "b"); ImpSyntax.Var (name_of_string "c"); ImpSyntax.Var (name_of_string "d")];
+      ImpSyntax.Call (name_of_string "ret") (name_of_string "cons") 
+        [ImpSyntax.Var (name_of_string "a"); ImpSyntax.Var (name_of_string "ret")];
+      ImpSyntax.Return (ImpSyntax.Var (name_of_string "ret"))]);
+   (name_of_string "cons5", [name_of_string "a"; name_of_string "b"; name_of_string "c"; name_of_string "d"; name_of_string "e"], list_Seq
+     [ImpSyntax.Call (name_of_string "ret") (name_of_string "cons4")
+        [ImpSyntax.Var (name_of_string "b"); ImpSyntax.Var (name_of_string "c"); 
+         ImpSyntax.Var (name_of_string "d"); ImpSyntax.Var (name_of_string "e")];
+      ImpSyntax.Call (name_of_string "ret") (name_of_string "cons") 
+        [ImpSyntax.Var (name_of_string "a"); ImpSyntax.Var (name_of_string "ret")];
+      ImpSyntax.Return (ImpSyntax.Var (name_of_string "ret"))])].
+
+Definition get_func_name (d: FunSyntax.defun): name :=
+  match d with
+  | FunSyntax.Defun n _ _ => N.to_nat n
+  end.
+
+Definition has_conflicting_names (defs: list FunSyntax.defun): bool :=
+  let reserved_names := name_of_string_N "main" :: map (fun '(n,_,_) => (N.of_nat n)) builtin in
+  List.existsb (fun d =>
+    List.existsb (N.eqb (N.of_nat (get_func_name d))) reserved_names
+  ) defs.
+
+Definition to_imp (p: FunSyntax.prog): option ImpSyntax.prog :=
+  match p with
+  | FunSyntax.Program defs main =>
+    if has_conflicting_names defs then None else
+    match to_funs (FunSyntax.Defun (name_of_string_N "main") [] main :: defs) with
+    | Some fs =>
+        Some (
+          ImpSyntax.Program
+            (map (fun '(n, vs, b) => ImpSyntax.Func n vs b) builtin ++ fs)
+        )
+    | None => None
+    end
+  end.
+
+Example fp_prog1 :=
+  FunSyntax.Program (@nil FunSyntax.defun) (
+    FunSyntax.Op FunSyntax.Add [FunSyntax.Const 1; FunSyntax.Const 2]
+  ).
+Compute (to_imp fp_prog1).
+
+Example fp_prog2 :=
+  FunSyntax.Program (@nil FunSyntax.defun) (
+    FunSyntax.Let 1
+      (FunSyntax.Op FunSyntax.Add [FunSyntax.Const 1; FunSyntax.Const 2])
+      (FunSyntax.Var 1)
+  ).
+Compute (to_imp fp_prog2).
+
+(* TODO: forward semantics preservation *)
